decidable

LeanYjs/Basic.lean
@@ -22,7 +22,20 @@ inductive YjsPtr : Type where
 | last : YjsPtr
 
 inductive YjsItem : Type where
-| item : (origin : YjsPtr) -> (rightOrigin : YjsPtr) -> ActorId -> A -> YjsItem
+| item (origin : YjsPtr) (rightOrigin : YjsPtr) : ActorId -> A -> YjsItem
+end
+
+mutual
+def YjsPtr.size {A : Type} (x : YjsPtr A) :=
+  match x with
+  | YjsPtr.itemPtr item => item.size + 1
+  | YjsPtr.first => 0
+  | YjsPtr.last => 0
+
+def YjsItem.size {A : Type} (item : YjsItem A) :=
+  match item with
+  | YjsItem.item origin rightOrigin _ _ =>
+    origin.size + rightOrigin.size + 2
 end
 
 instance : BEq ActorId where
@@ -62,38 +75,47 @@ def YjsItem.rightOrigin {A : Type} : YjsItem A -> YjsPtr A
 def YjsItem.id {A : Type} : YjsItem A -> ActorId
 | YjsItem.item _ _ id _ => id
 
-inductive YjsLessThan {A : Type} : YjsPtr A -> YjsPtr A -> Prop where
-| ltFirst: forall l r id (c : A), YjsLessThan (YjsPtr.first) (YjsItem.item l r id c)
-| ltLast: forall l r id (c : A), YjsLessThan (YjsItem.item l r id c) (YjsPtr.last)
-| ltL1 : forall l r id c, YjsLessThan l (YjsItem.item l r id c)
-| ltR1 : forall l r id c, YjsLessThan (YjsItem.item l r id c) r
+mutual
+inductive YjsLt {A : Type} : YjsPtr A -> YjsPtr A -> Prop where
+| ltFirst : forall item, YjsLt (YjsPtr.first) (YjsPtr.itemPtr item)
+| ltLast : forall item, YjsLt (YjsPtr.itemPtr item) (YjsPtr.last)
+| ltFirstLast: YjsLt (YjsPtr.first) (YjsPtr.last)
+| ltL1 : forall l r id c, YjsLt l (YjsItem.item l r id c)
+| ltR1 : forall l r id c, YjsLt (YjsItem.item l r id c) r
 | ltL2 : forall l1 r1 id1 l2 r2 id2 (c1 c2 : A),
-  YjsLessThan (YjsItem.item l1 r1 id1 c1) l2 -> YjsLessThan (YjsItem.item l1 r1 id1 c1) (YjsItem.item l2 r2 id2 c2)
+  YjsLeq (YjsItem.item l1 r1 id1 c1) l2
+  -> YjsLt (YjsItem.item l1 r1 id1 c1) (YjsItem.item l2 r2 id2 c2)
 | ltR2 : forall l1 r1 id1 l2 r2 id2 (c1 c2 : A),
-  YjsLessThan r1 (YjsItem.item l2 r2 id2 c2) -> YjsLessThan (YjsItem.item l1 r1 id1 c1) (YjsItem.item l2 r2 id2 c2)
-| ltOriginDiff : forall l1 l2 (r1 r2 : YjsItem A) id1 id2 c1 c2,
-  YjsLessThan l2 l1
-  -> YjsLessThan (YjsItem.item l1 r1 id1 c1) r2
-  -> YjsLessThan l1 (YjsItem.item l2 r2 id2 c2)
-  -> YjsLessThan (YjsItem.item l2 r2 id2 c2) r1
-  -> YjsLessThan (YjsItem.item l1 r1 id1 c1) (YjsItem.item l2 r2 id2 c2)
+  YjsLeq r1 (YjsItem.item l2 r2 id2 c2)
+  -> YjsLt (YjsItem.item l1 r1 id1 c1) (YjsItem.item l2 r2 id2 c2)
+| ltOriginDiff : forall l1 l2 r1 r2 id1 id2 c1 c2,
+  YjsLt l2 l1
+  -> YjsLt (YjsItem.item l1 r1 id1 c1) r2
+  -> YjsLt l1 (YjsItem.item l2 r2 id2 c2)
+  -> YjsLt (YjsItem.item l2 r2 id2 c2) r1
+  -> YjsLt (YjsItem.item l1 r1 id1 c1) (YjsItem.item l2 r2 id2 c2)
 | ltOriginSame : forall l r1 r2 id1 id2 (c1 c2 : A),
-  YjsLessThan (YjsItem.item l r1 id1 c1) r2
-  -> YjsLessThan (YjsItem.item l r2 id2 c2) r1
+  YjsLt (YjsItem.item l r1 id1 c1) r2
+  -> YjsLt (YjsItem.item l r2 id2 c2) r1
   -> id1 < id2
-  -> YjsLessThan (YjsItem.item l r1 id1 c1) (YjsItem.item l r2 id2 c2)
+  -> YjsLt (YjsItem.item l r1 id1 c1) (YjsItem.item l r2 id2 c2)
+
+inductive YjsLeq {A : Type} : YjsPtr A -> YjsPtr A -> Prop where
+  | ltLeq x y : YjsLt x y -> YjsLeq x y
+  | ltEq x y : x = y -> YjsLeq x y
+end
 
 namespace ex1
   open Nat
   def item1 : YjsPtr Nat := YjsItem.item YjsPtr.first YjsPtr.last 1 1
   def item2 : YjsPtr Nat := YjsItem.item YjsPtr.first YjsPtr.last 2 2
 
-  example : YjsLessThan item1 item2 :=
+  example : YjsLt item1 item2 :=
   by
     unfold item1 item2
-    apply YjsLessThan.ltOriginSame <;> try rfl
-    . apply YjsLessThan.ltLast
-    . apply YjsLessThan.ltLast
+    apply YjsLt.ltOriginSame <;> try rfl
+    . apply YjsLt.ltLast
+    . apply YjsLt.ltLast
     simp [ActorId]
 end ex1
 
@@ -102,14 +124,174 @@ namespace ex2
   def item1 : YjsPtr Nat := YjsItem.item YjsPtr.first YjsPtr.last 1 1
   def item2 : YjsPtr Nat := YjsItem.item YjsPtr.first item0 2 2
 
-  example : YjsLessThan item2 item1 :=
+  example : YjsLt item2 item1 :=
   by
-    apply YjsLessThan.ltR2
-    . apply YjsLessThan.ltOriginSame
-      apply YjsLessThan.ltLast
-      apply YjsLessThan.ltLast
+    apply YjsLt.ltR2
+    . apply YjsLeq.ltLeq
+      apply YjsLt.ltOriginSame
+      apply YjsLt.ltLast
+      apply YjsLt.ltLast
       simp [ActorId]
 end ex2
 
-theorem order_is_strict_total: IsStrictTotalOrder _ (@YjsLessThan A) := by
+mutual
+lemma yjs_decidable1 (A : Type) : forall (x y : YjsPtr A), YjsLeq x y ∨ YjsLt y x :=
+  fun (x : YjsPtr A) (y : YjsPtr A) =>
+  match x with
+  | YjsPtr.first =>
+    match y with
+    | YjsPtr.first => by
+      left
+      right
+      eq_refl
+    | YjsPtr.last => by
+      left
+      left
+      apply YjsLt.ltFirstLast
+    | YjsPtr.itemPtr item => by
+      left
+      left
+      apply YjsLt.ltFirst
+  | YjsPtr.last =>
+    match y with
+    | YjsPtr.first => by
+      right
+      apply YjsLt.ltFirstLast
+    | YjsPtr.last => by
+      left
+      right
+      eq_refl
+    | YjsPtr.itemPtr item => by
+      right
+      apply YjsLt.ltLast
+  | YjsPtr.itemPtr item =>
+    match y with
+    | YjsPtr.first => by
+      right
+      apply YjsLt.ltFirst
+    | YjsPtr.last => by
+      left
+      apply YjsLeq.ltLeq
+      apply YjsLt.ltLast
+    | YjsPtr.itemPtr item' =>
+      have h : item.size + item'.size < (YjsPtr.itemPtr item).size + (YjsPtr.itemPtr item').size := by
+        simp!
+        omega
+      yjs_decidable2 (x := item) (y := item')
+termination_by x y => x.size + y.size
+
+lemma yjs_decidable2 A : forall (x y : YjsItem A), @YjsLeq A x y ∨ @YjsLt A y x :=
+  fun (x y : YjsItem A) => by
+  cases x with
+  | item l1 r1 id1 c1 =>
+    cases y with
+    | item l2 r2 id2 c2 =>
+      have h : (YjsPtr.itemPtr (YjsItem.item l1 r1 id1 c1)).size + l2.size <
+        (YjsItem.item l1 r1 id1 c1).size + (YjsItem.item l2 r2 id2 c2).size := by
+        simp!
+        omega
+      cases yjs_decidable1 _ (YjsItem.item l1 r1 id1 c1) l2 with
+      | inl hlt =>
+        left
+        left
+        apply YjsLt.ltL2
+        assumption
+      | inr hlt1 =>
+        have h : r2.size + (YjsPtr.itemPtr (YjsItem.item l1 r1 id1 c1)).size <
+          (YjsItem.item l1 r1 id1 c1).size + (YjsItem.item l2 r2 id2 c2).size := by
+          simp!
+          omega
+        cases yjs_decidable1 _ r2 (YjsItem.item l1 r1 id1 c1) with
+        | inl hlt2 =>
+          right
+          apply YjsLt.ltR2
+          assumption
+        | inr hlt2 =>
+          have h : l1.size + (YjsPtr.itemPtr (YjsItem.item l2 r2 id2 c2)).size <
+            (YjsItem.item l1 r1 id1 c1).size + (YjsItem.item l2 r2 id2 c2).size := by
+            simp!
+            omega
+          cases yjs_decidable1 _ (YjsItem.item l2 r2 id2 c2) l1 with
+          | inl hlt3 =>
+            right
+            apply YjsLt.ltL2
+            assumption
+          | inr hlt3 =>
+            have h : r1.size + (YjsPtr.itemPtr (YjsItem.item l2 r2 id2 c2)).size <
+              (YjsItem.item l1 r1 id1 c1).size + (YjsItem.item l2 r2 id2 c2).size := by
+              simp!
+              omega
+            cases yjs_decidable1 _ r1 (YjsItem.item l2 r2 id2 c2) with
+            | inl hlt4 =>
+              left
+              apply YjsLeq.ltLeq
+              apply YjsLt.ltR2
+              assumption
+            | inr hlt4 =>
+              have h : l1.size + l2.size <
+                (YjsItem.item l1 r1 id1 c1).size + (YjsItem.item l2 r2 id2 c2).size := by
+                simp!
+                omega
+              cases yjs_decidable1 _ l1 l2 with
+              | inl hlt5 =>
+                cases hlt5 with
+                | ltEq _ _ heq =>
+                  rw [heq]
+                  cases Nat.decLt id1 id2 with
+                  | isTrue h =>
+                    left
+                    apply YjsLeq.ltLeq
+                    apply YjsLt.ltOriginSame <;> try assumption
+                    rw [<-heq] <;> assumption
+                  | isFalse h =>
+                    have h' : id1 = id2 ∨ id2 < id1 := by
+                      unfold ActorId
+                      omega
+                    cases h' with
+                    | inl heq =>
+                      sorry -- id1 = id2なのでconcurrentにはなりえない
+                    | inr hlt6 =>
+                      right
+                      apply YjsLt.ltOriginSame <;> try assumption
+                      rw [<-heq]
+                      assumption
+                | ltLeq _ _ hlt6 =>
+                  right
+                  apply YjsLt.ltOriginDiff <;> assumption
+              | inr hlt5 =>
+                left
+                apply YjsLeq.ltLeq
+                apply YjsLt.ltOriginDiff <;> assumption
+termination_by x y => x.size + y.size
+end
+
+lemma yjs_lt_invert (x y : YjsItem A) (x' y' : YjsPtr A) :
+  x = x' -> y = y' -> @YjsLt A x' y' -> YjsLeq x (y.origin) ∨ YjsLeq (x.origin) (y.origin) := by
+  intros hx hy hlt
+  induction hlt
+  . injection hx
+  . injection hy
+  . left
+    right
+    injection hy with hy
+    rw [hx, hy]
+    eq_refl
+  . left
+    left
+    injection hx with hx
+    rw [hx, <-hy]
+    sorry -- item < item.rightOrigin.originが必要
+  . left
+    left
+    injections hx hy
+    rw [hx, hy]
+    simp!
+    assumption
+  . injections hx hy
+    rw [hx, hy]
+    simp!
+
+
+
+theorem order_is_strict_total: IsStrictTotalOrder _ (@YjsLt A) := by
   sorry
